WP rules - AddSubLt

theories/rules/rules_AddSubLt.v
@@ -15,7 +15,7 @@ Section cap_lang_rules.
   Implicit Types r : RegName.
   Implicit Types v : cap_lang.val. 
   Implicit Types w : Word.
-  Implicit Types reg : gmap RegName Word.
+  Implicit Types reg : gmap (CoreN * RegName) Word.
   Implicit Types ms : gmap Addr Word.
 
   Definition denote (i: instr) (n1 n2: Z): Z :=
@@ -38,44 +38,56 @@ Section cap_lang_rules.
     intros HH. destruct_or! HH; subst i; reflexivity.
   Qed.
 
-  Inductive AddSubLt_failure (i: instr) (regs: Reg) (dst: RegName) (rv1 rv2: Z + RegName) (regs': Reg) :=
-  | AddSubLt_fail_nonconst1:
-      z_of_argument regs rv1 = None ->
-      AddSubLt_failure i regs dst rv1 rv2 regs'
-  | AddSubLt_fail_nonconst2:
-      z_of_argument regs rv2 = None ->
-      AddSubLt_failure i regs dst rv1 rv2 regs'
-  | AddSubLt_fail_incrPC n1 n2:
-      z_of_argument regs rv1 = Some n1 ->
-      z_of_argument regs rv2 = Some n2 ->
-      incrementPC (<[ dst := WInt (denote i n1 n2) ]> regs) = None ->
-      AddSubLt_failure i regs dst rv1 rv2 regs'.
+  Lemma regs_of_core_is_AddSubLt it r arg1 arg2 i :
+    is_AddSubLt it r arg1 arg2 →
+    regs_of_core it i = {[ (i,r) ]} ∪
+                          set_map (λ r, (i, r)) (regs_of_argument arg1) ∪
+                          set_map (λ r, (i, r)) (regs_of_argument arg2).
+  Proof.
+    intros HH.
+    rewrite /regs_of_core.
+    erewrite regs_of_is_AddSubLt ; eauto.
+    set_solver.
+  Qed.
 
-  Inductive AddSubLt_spec (i: instr) (regs: Reg) (dst: RegName) (rv1 rv2: Z + RegName) (regs': Reg): cap_lang.val -> Prop :=
+  Inductive AddSubLt_failure (it: instr) (i : CoreN) (regs: Reg) (dst: RegName) (rv1 rv2: Z + RegName) (regs': Reg) :=
+  | AddSubLt_fail_nonconst1:
+      z_of_argument regs i rv1 = None ->
+      AddSubLt_failure it i regs dst rv1 rv2 regs'
+  | AddSubLt_fail_nonconst2:
+      z_of_argument regs i rv2 = None ->
+      AddSubLt_failure it i regs dst rv1 rv2 regs'
+  | AddSubLt_fail_incrPC n1 n2:
+      z_of_argument regs i rv1 = Some n1 ->
+      z_of_argument regs i rv2 = Some n2 ->
+      incrementPC (<[ (i, dst) := WInt (denote it n1 n2) ]> regs) i = None ->
+      AddSubLt_failure it i regs dst rv1 rv2 regs'.
+
+  Inductive AddSubLt_spec (it: instr) (i : CoreN) (regs: Reg) (dst: RegName) (rv1 rv2: Z + RegName) (regs': Reg): cap_lang.val -> Prop :=
   | AddSubLt_spec_success n1 n2:
-      z_of_argument regs rv1 = Some n1 ->
-      z_of_argument regs rv2 = Some n2 ->
-      incrementPC (<[ dst := WInt (denote i n1 n2) ]> regs) = Some regs' ->
-      AddSubLt_spec i regs dst rv1 rv2 regs' NextIV
+      z_of_argument regs i rv1 = Some n1 ->
+      z_of_argument regs i rv2 = Some n2 ->
+      incrementPC (<[ (i, dst) := WInt (denote it n1 n2) ]> regs) i = Some regs' ->
+      AddSubLt_spec it i regs dst rv1 rv2 regs' (i, NextIV)
   | AddSubLt_spec_failure:
-      AddSubLt_failure i regs dst rv1 rv2 regs' ->
-      AddSubLt_spec i regs dst rv1 rv2 regs' FailedV.
+      AddSubLt_failure it i regs dst rv1 rv2 regs' ->
+      AddSubLt_spec it i regs dst rv1 rv2 regs' (i, FailedV).
 
   Local Ltac iFail Hcont get_fail_case :=
     cbn; iFrame; iApply Hcont; iFrame; iPureIntro;
     econstructor; eapply get_fail_case; eauto.
 
-  Lemma wp_AddSubLt Ep i pc_p pc_b pc_e pc_a w dst arg1 arg2 regs :
-    decodeInstrW w = i →
-    is_AddSubLt i dst arg1 arg2 →
+  Lemma wp_AddSubLt Ep i it pc_p pc_b pc_e pc_a w dst arg1 arg2 regs :
+    decodeInstrW w = it →
+    is_AddSubLt it dst arg1 arg2 →
     isCorrectPC (WCap pc_p pc_b pc_e pc_a) →
-    regs !! PC = Some (WCap pc_p pc_b pc_e pc_a) →
-    regs_of i ⊆ dom _ regs →
+    regs !! (i, PC) = Some (WCap pc_p pc_b pc_e pc_a) →
+    regs_of_core it i ⊆ dom _ regs →
     {{{ ▷ pc_a ↦ₐ w ∗
         ▷ [∗ map] k↦y ∈ regs, k ↦ᵣ y }}}
-      Instr Executable @ Ep
+      (i, Instr Executable) @ Ep
     {{{ regs' retv, RET retv;
-        ⌜ AddSubLt_spec (decodeInstrW w) regs dst arg1 arg2 regs' retv ⌝ ∗
+        ⌜ AddSubLt_spec (decodeInstrW w) i regs dst arg1 arg2 regs' retv ⌝ ∗
           pc_a ↦ₐ w ∗
           [∗ map] k↦y ∈ regs', k ↦ᵣ y }}}.
   Proof.
@@ -89,18 +101,18 @@ Section cap_lang_rules.
     iModIntro. iSplitR. by iPureIntro; apply normal_always_head_reducible.
     iNext. iIntros (e2 σ2 efs Hpstep).
     apply prim_step_exec_inv in Hpstep as (-> & -> & (c & -> & Hstep)).
-    iSplitR; auto. eapply step_exec_inv in Hstep; eauto.
+    iSplitR; auto. eapply core_step_exec_inv in Hstep; eauto.
     unfold exec in Hstep.
 
     specialize (indom_regs_incl _ _ _ Dregs Hregs) as Hri.
-    erewrite regs_of_is_AddSubLt in Hri, Dregs; eauto.
-    destruct (Hri dst) as [wdst [H'dst Hdst]]. by set_solver+.
+    erewrite regs_of_core_is_AddSubLt in Hri, Dregs; eauto.
+    destruct (Hri i dst) as [wdst [H'dst Hdst]]. by set_solver+.
 
-    destruct (z_of_argument regs arg1) as [n1|] eqn:Hn1;
+    destruct (z_of_argument regs i arg1) as [n1|] eqn:Hn1;
       pose proof Hn1 as Hn1'; cycle 1.
     (* Failure: arg1 is not an integer *)
     { unfold z_of_argument in Hn1. destruct arg1 as [| r0]; [ congruence |].
-      destruct (Hri r0) as [r0v [Hr'0 Hr0]]. by unfold regs_of_argument; set_solver+.
+      destruct (Hri i r0) as [r0v [Hr'0 Hr0]]. by unfold regs_of_argument; set_solver+.
       rewrite Hr'0 in Hn1. destruct r0v as [| ? ? ? ? ]; [ congruence |].
       assert (c = Failed ∧ σ2 = (r, m)) as (-> & ->).
       { destruct_or! Hinstr; rewrite Hinstr /= in Hstep.
@@ -108,11 +120,11 @@ Section cap_lang_rules.
       iFail "Hφ" AddSubLt_fail_nonconst1. }
     apply (z_of_arg_mono _ r) in Hn1; auto.
 
-    destruct (z_of_argument regs arg2) as [n2|] eqn:Hn2;
+    destruct (z_of_argument regs i arg2) as [n2|] eqn:Hn2;
       pose proof Hn2 as Hn2'; cycle 1.
     (* Failure: arg2 is not an integer *)
     { unfold z_of_argument in Hn2. destruct arg2 as [| r0]; [ congruence |].
-      destruct (Hri r0) as [r0v [Hr'0 Hr0]]. by unfold regs_of_argument; set_solver+.
+      destruct (Hri i r0) as [r0v [Hr'0 Hr0]]. by unfold regs_of_argument; set_solver+.
       rewrite Hr'0 in Hn2. destruct r0v as [| ? ? ? ? ]; [ congruence |].
       assert (c = Failed ∧ σ2 = (r, m)) as (-> & ->).
       { destruct_or! Hinstr; rewrite Hinstr /= Hn1 in Hstep; cbn in Hstep.
@@ -120,12 +132,12 @@ Section cap_lang_rules.
       iFail "Hφ" AddSubLt_fail_nonconst2. }
     apply (z_of_arg_mono _ r) in Hn2; auto.
 
-    assert (exec_opt i (r, m) = updatePC (update_reg (r, m) dst (WInt (denote i n1 n2)))) as HH.
+    assert (exec_opt it i (r, m) = updatePC i (update_reg (r, m) i dst (WInt (denote it n1 n2)))) as HH.
     { all: destruct_or! Hinstr; rewrite Hinstr /= /update_reg /= in Hstep |- *; auto.
       all: by rewrite Hn1 Hn2; cbn. }
     rewrite HH in Hstep. rewrite /update_reg /= in Hstep.
 
-    destruct (incrementPC (<[ dst := WInt (denote i n1 n2) ]> regs))
+    destruct (incrementPC (<[ (i, dst) := WInt (denote it n1 n2) ]> regs) i)
       as [regs'|] eqn:Hregs'; pose proof Hregs' as H'regs'; cycle 1.
     (* Failure: Cannot increment PC *)
     { apply incrementPC_fail_updatePC with (m:=m) in Hregs'.
@@ -139,373 +151,405 @@ Section cap_lang_rules.
 
     (* Success *)
 
-    eapply (incrementPC_success_updatePC _ m) in Hregs'
+    eapply (incrementPC_success_updatePC _ i m) in Hregs'
       as (p' & g' & b' & e' & a'' & a_pc' & HPC'' & HuPC & ->).
     eapply updatePC_success_incl with (m':=m) in HuPC. 2: by eapply insert_mono; eauto. rewrite HuPC in Hstep.
     simplify_pair_eq. iFrame.
-    iMod ((gen_heap_update_inSepM _ _ dst) with "Hr Hmap") as "[Hr Hmap]"; eauto.
-    iMod ((gen_heap_update_inSepM _ _ PC) with "Hr Hmap") as "[Hr Hmap]"; eauto.
+    iMod ((gen_heap_update_inSepM _ _ (i, dst)) with "Hr Hmap") as "[Hr Hmap]"; eauto.
+    iMod ((gen_heap_update_inSepM _ _ (i, PC)) with "Hr Hmap") as "[Hr Hmap]"; eauto.
     iFrame. iModIntro. iApply "Hφ". iFrame. iPureIntro. econstructor; eauto.
   Qed.
 
   (* Derived specifications *)
 
-  Lemma wp_add_sub_lt_success_z_z E dst pc_p pc_b pc_e pc_a w wdst ins n1 n2 pc_a' :
+  Lemma wp_add_sub_lt_success_z_z E i dst pc_p pc_b pc_e pc_a w wdst ins n1 n2 pc_a' :
     decodeInstrW w = ins →
     is_AddSubLt ins dst (inl n1) (inl n2) →
     (pc_a + 1)%a = Some pc_a' →
     isCorrectPC (WCap pc_p pc_b pc_e pc_a) ->
 
-    {{{ PC ↦ᵣ WCap pc_p pc_b pc_e pc_a
+    {{{ (i, PC) ↦ᵣ WCap pc_p pc_b pc_e pc_a
         ∗ pc_a ↦ₐ w
-        ∗ dst ↦ᵣ wdst
+        ∗ (i, dst) ↦ᵣ wdst
     }}}
-      Instr Executable @ E
-      {{{ RET NextIV;
-          PC ↦ᵣ WCap pc_p pc_b pc_e pc_a'
+      (i, Instr Executable) @ E
+      {{{ RET (i, NextIV);
+          (i, PC) ↦ᵣ WCap pc_p pc_b pc_e pc_a'
           ∗ pc_a ↦ₐ w
-          ∗ dst ↦ᵣ WInt (denote ins n1 n2)
+          ∗ (i, dst) ↦ᵣ WInt (denote ins n1 n2)
       }}}.
   Proof.
     iIntros (Hdecode Hinstr Hpc_a Hvpc ϕ) "(HPC & Hpc_a & Hdst) Hφ".
     iDestruct (map_of_regs_2 with "HPC Hdst") as "[Hmap %]".
     iApply (wp_AddSubLt with "[$Hmap Hpc_a]"); eauto; simplify_map_eq; eauto.
-    by erewrite regs_of_is_AddSubLt; eauto; rewrite !dom_insert; set_solver+.
+    by erewrite regs_of_core_is_AddSubLt; eauto; rewrite !dom_insert; set_solver+.
     iNext. iIntros (regs' retv) "(#Hspec & Hpc_a & Hmap)". iDestruct "Hspec" as %Hspec.
 
     destruct Hspec as [| * Hfail].
     { (* Success *)
-      iApply "Hφ". iFrame. incrementPC_inv; simplify_map_eq.
-      rewrite insert_commute // insert_insert insert_commute // insert_insert.
+      iApply "Hφ". iFrame. incrementPC_inv; simplify_map_eq by simplify_pair_eq.
+      rewrite insert_commute ; simplify_pair_eq.
+      rewrite insert_insert insert_commute ; simplify_pair_eq.
+      rewrite insert_insert.
       iDestruct (regs_of_map_2 with "Hmap") as "[? ?]"; eauto; iFrame. }
     { (* Failure (contradiction) *)
-      destruct Hfail; try incrementPC_inv; simplify_map_eq; eauto. congruence. }
+      destruct Hfail; try incrementPC_inv; simplify_map_eq by simplify_pair_eq; eauto. congruence. }
   Qed.
 
-  Lemma wp_add_sub_lt_success_r_z E dst pc_p pc_b pc_e pc_a w wdst ins r1 n1 n2 pc_a' :
+  Lemma wp_add_sub_lt_success_r_z E i dst pc_p pc_b pc_e pc_a w wdst ins r1 n1 n2 pc_a' :
     decodeInstrW w = ins →
     is_AddSubLt ins dst (inr r1) (inl n2) →
     (pc_a + 1)%a = Some pc_a' →
     isCorrectPC (WCap pc_p pc_b pc_e pc_a) ->
 
-    {{{ PC ↦ᵣ WCap pc_p pc_b pc_e pc_a
+    {{{ (i, PC) ↦ᵣ WCap pc_p pc_b pc_e pc_a
         ∗ pc_a ↦ₐ w
-        ∗ r1 ↦ᵣ WInt n1
-        ∗ dst ↦ᵣ wdst
+        ∗ (i, r1) ↦ᵣ WInt n1
+        ∗ (i, dst) ↦ᵣ wdst
     }}}
-      Instr Executable @ E
-      {{{ RET NextIV;
-          PC ↦ᵣ WCap pc_p pc_b pc_e pc_a'
+      (i, Instr Executable) @ E
+      {{{ RET (i, NextIV);
+          (i, PC) ↦ᵣ WCap pc_p pc_b pc_e pc_a'
           ∗ pc_a ↦ₐ w
-          ∗ r1 ↦ᵣ WInt n1
-          ∗ dst ↦ᵣ WInt (denote ins n1 n2)
+          ∗ (i, r1) ↦ᵣ WInt n1
+          ∗ (i, dst) ↦ᵣ WInt (denote ins n1 n2)
       }}}.
   Proof.
     iIntros (Hdecode Hinstr Hpc_a Hvpc ϕ) "(HPC & Hpc_a & Hr1 & Hdst) Hφ".
     iDestruct (map_of_regs_3 with "HPC Hr1 Hdst") as "[Hmap (%&%&%)]".
-    iApply (wp_AddSubLt with "[$Hmap Hpc_a]"); eauto; simplify_map_eq; eauto.
-    by erewrite regs_of_is_AddSubLt; eauto; rewrite !dom_insert; set_solver+.
+    iApply (wp_AddSubLt with "[$Hmap Hpc_a]"); eauto; simplify_map_eq by simplify_pair_eq; eauto.
+    by erewrite regs_of_core_is_AddSubLt; eauto; rewrite !dom_insert; set_solver+.
     iNext. iIntros (regs' retv) "(#Hspec & Hpc_a & Hmap)". iDestruct "Hspec" as %Hspec.
 
     destruct Hspec as [| * Hfail].
     { (* Success *)
-      iApply "Hφ". iFrame. incrementPC_inv; simplify_map_eq.
-      rewrite (insert_commute _ PC dst) // insert_insert (insert_commute _ r1 dst) //
-              (insert_commute _ dst PC) // insert_insert.
+      iApply "Hφ". iFrame. incrementPC_inv; simplify_map_eq by simplify_pair_eq.
+      rewrite (insert_commute _ (i, PC) (i, dst)) ; simplify_pair_eq.
+      rewrite insert_insert.
+      rewrite (insert_commute _ (i, r1) (i, dst)) ; simplify_pair_eq.
+      rewrite (insert_commute _ (i, dst) (i, PC)) ; simplify_pair_eq.
+      rewrite insert_insert.
       iDestruct (regs_of_map_3 with "Hmap") as "(?&?&?)"; eauto; iFrame. }
     { (* Failure (contradiction) *)
-      destruct Hfail; try incrementPC_inv; simplify_map_eq; eauto. congruence. }
+      destruct Hfail; try incrementPC_inv; simplify_map_eq by simplify_pair_eq; eauto. congruence. }
   Qed.
 
-  Lemma wp_add_sub_lt_success_z_r E dst pc_p pc_b pc_e pc_a w wdst ins n1 r2 n2 pc_a' :
+  Lemma wp_add_sub_lt_success_z_r E i dst pc_p pc_b pc_e pc_a w wdst ins n1 r2 n2 pc_a' :
     decodeInstrW w = ins →
     is_AddSubLt ins dst (inl n1) (inr r2) →
     (pc_a + 1)%a = Some pc_a' →
     isCorrectPC (WCap pc_p pc_b pc_e pc_a) ->
 
-    {{{ PC ↦ᵣ WCap pc_p pc_b pc_e pc_a
+    {{{ (i, PC) ↦ᵣ WCap pc_p pc_b pc_e pc_a
         ∗ pc_a ↦ₐ w
-        ∗ r2 ↦ᵣ WInt n2
-        ∗ dst ↦ᵣ wdst
+        ∗ (i, r2) ↦ᵣ WInt n2
+        ∗ (i, dst) ↦ᵣ wdst
     }}}
-      Instr Executable @ E
-      {{{ RET NextIV;
-          PC ↦ᵣ WCap pc_p pc_b pc_e pc_a'
+      (i, Instr Executable) @ E
+      {{{ RET (i, NextIV);
+          (i, PC) ↦ᵣ WCap pc_p pc_b pc_e pc_a'
           ∗ pc_a ↦ₐ w
-          ∗ r2 ↦ᵣ WInt n2
-          ∗ dst ↦ᵣ WInt (denote ins n1 n2)
+          ∗ (i, r2) ↦ᵣ WInt n2
+          ∗ (i, dst) ↦ᵣ WInt (denote ins n1 n2)
       }}}.
   Proof.
     iIntros (Hdecode Hinstr Hpc_a Hvpc ϕ) "(HPC & Hpc_a & Hr2 & Hdst) Hφ".
     iDestruct (map_of_regs_3 with "HPC Hr2 Hdst") as "[Hmap (%&%&%)]".
-    iApply (wp_AddSubLt with "[$Hmap Hpc_a]"); eauto; simplify_map_eq; eauto.
-    by erewrite regs_of_is_AddSubLt; eauto; rewrite !dom_insert; set_solver+.
+    iApply (wp_AddSubLt with "[$Hmap Hpc_a]"); eauto; simplify_map_eq by simplify_pair_eq; eauto.
+    by erewrite regs_of_core_is_AddSubLt; eauto; rewrite !dom_insert; set_solver+.
     iNext. iIntros (regs' retv) "(#Hspec & Hpc_a & Hmap)". iDestruct "Hspec" as %Hspec.
 
     destruct Hspec as [| * Hfail].
     { (* Success *)
-      iApply "Hφ". iFrame. incrementPC_inv; simplify_map_eq.
-      rewrite (insert_commute _ PC dst) // insert_insert (insert_commute _ r2 dst) //
-              (insert_commute _ dst PC) // insert_insert.
+      iApply "Hφ". iFrame. incrementPC_inv; simplify_map_eq by simplify_pair_eq.
+      rewrite (insert_commute _ (i, PC) (i, dst)) ; simplify_pair_eq.
+      rewrite insert_insert.
+      rewrite (insert_commute _ (i, r2) (i, dst)) ; simplify_pair_eq.
+      rewrite (insert_commute _ (i, dst) (i, PC)) ; simplify_pair_eq.
+      rewrite insert_insert.
       iDestruct (regs_of_map_3 with "Hmap") as "(?&?&?)"; eauto; iFrame. }
     { (* Failure (contradiction) *)
-      destruct Hfail; try incrementPC_inv; simplify_map_eq; eauto. congruence. }
+      destruct Hfail; try incrementPC_inv; simplify_map_eq by simplify_pair_eq; eauto. congruence. }
   Qed.
 
-  Lemma wp_add_sub_lt_success_r_r E dst pc_p pc_b pc_e pc_a w wdst ins r1 n1 r2 n2 pc_a' :
+  Lemma wp_add_sub_lt_success_r_r E i dst pc_p pc_b pc_e pc_a w wdst ins r1 n1 r2 n2 pc_a' :
     decodeInstrW w = ins →
     is_AddSubLt ins dst (inr r1) (inr r2) →
     (pc_a + 1)%a = Some pc_a' →
     isCorrectPC (WCap pc_p pc_b pc_e pc_a) ->
 
-    {{{ PC ↦ᵣ WCap pc_p pc_b pc_e pc_a
+    {{{ (i, PC) ↦ᵣ WCap pc_p pc_b pc_e pc_a
         ∗ pc_a ↦ₐ w
-        ∗ r1 ↦ᵣ WInt n1
-        ∗ r2 ↦ᵣ WInt n2
-        ∗ dst ↦ᵣ wdst
+        ∗ (i, r1) ↦ᵣ WInt n1
+        ∗ (i, r2) ↦ᵣ WInt n2
+        ∗ (i, dst) ↦ᵣ wdst
     }}}
-      Instr Executable @ E
-      {{{ RET NextIV;
-          PC ↦ᵣ WCap pc_p pc_b pc_e pc_a'
+      (i, Instr Executable) @ E
+      {{{ RET (i, NextIV);
+          (i, PC) ↦ᵣ WCap pc_p pc_b pc_e pc_a'
           ∗ pc_a ↦ₐ w
-          ∗ r1 ↦ᵣ WInt n1
-          ∗ r2 ↦ᵣ WInt n2
-          ∗ dst ↦ᵣ WInt (denote ins n1 n2)
+          ∗ (i, r1) ↦ᵣ WInt n1
+          ∗ (i, r2) ↦ᵣ WInt n2
+          ∗ (i, dst) ↦ᵣ WInt (denote ins n1 n2)
       }}}.
   Proof.
     iIntros (Hdecode Hinstr Hpc_a Hvpc ϕ) "(HPC & Hpc_a & Hr1 & Hr2 & Hdst) Hφ".
     iDestruct (map_of_regs_4 with "HPC Hr1 Hr2 Hdst") as "[Hmap (%&%&%&%&%&%)]".
-    iApply (wp_AddSubLt with "[$Hmap Hpc_a]"); eauto; simplify_map_eq; eauto.
-    by erewrite regs_of_is_AddSubLt; eauto; rewrite !dom_insert; set_solver+.
+    iApply (wp_AddSubLt with "[$Hmap Hpc_a]"); eauto; simplify_map_eq by simplify_pair_eq; eauto.
+    by erewrite regs_of_core_is_AddSubLt; eauto; rewrite !dom_insert; set_solver+.
     iNext. iIntros (regs' retv) "(#Hspec & Hpc_a & Hmap)". iDestruct "Hspec" as %Hspec.
 
     destruct Hspec as [| * Hfail].
     { (* Success *)
-      iApply "Hφ". iFrame. incrementPC_inv; simplify_map_eq.
-      rewrite (insert_commute _ PC dst) // insert_insert (insert_commute _ r2 dst) //
-              (insert_commute _ r1 dst) // (insert_commute _ PC dst) // insert_insert.
+      iApply "Hφ". iFrame. incrementPC_inv; simplify_map_eq by simplify_pair_eq.
+      rewrite (insert_commute _ (i, PC) (i, dst)) ; simplify_pair_eq.
+      rewrite insert_insert.
+      rewrite (insert_commute _ (i, r2) (i, dst)) ; simplify_pair_eq.
+      rewrite (insert_commute _ (i, r1) (i, dst)) ; simplify_pair_eq.
+      rewrite (insert_commute _ (i, PC) (i, dst)) ; simplify_pair_eq.
+      rewrite insert_insert.
       iDestruct (regs_of_map_4 with "Hmap") as "(?&?&?&?)"; eauto; iFrame. }
     { (* Failure (contradiction) *)
-      destruct Hfail; try incrementPC_inv; simplify_map_eq; eauto. congruence. }
+      destruct Hfail; try incrementPC_inv; simplify_map_eq by simplify_pair_eq; eauto. congruence. }
   Qed.
 
-  Lemma wp_add_sub_lt_success_r_r_same E dst pc_p pc_b pc_e pc_a w wdst ins r n pc_a' :
+  Lemma wp_add_sub_lt_success_r_r_same E i dst pc_p pc_b pc_e pc_a w wdst ins r n pc_a' :
     decodeInstrW w = ins →
     is_AddSubLt ins dst (inr r) (inr r) →
     (pc_a + 1)%a = Some pc_a' →
     isCorrectPC (WCap pc_p pc_b pc_e pc_a) ->
 
-    {{{ PC ↦ᵣ WCap pc_p pc_b pc_e pc_a
+    {{{ (i, PC) ↦ᵣ WCap pc_p pc_b pc_e pc_a
         ∗ pc_a ↦ₐ w
-        ∗ r ↦ᵣ WInt n
-        ∗ dst ↦ᵣ wdst
+        ∗ (i, r) ↦ᵣ WInt n
+        ∗ (i, dst) ↦ᵣ wdst
     }}}
-      Instr Executable @ E
-      {{{ RET NextIV;
-          PC ↦ᵣ WCap pc_p pc_b pc_e pc_a'
+      (i, Instr Executable) @ E
+      {{{ RET (i, NextIV);
+          (i, PC) ↦ᵣ WCap pc_p pc_b pc_e pc_a'
           ∗ pc_a ↦ₐ w
-          ∗ r ↦ᵣ WInt n
-          ∗ dst ↦ᵣ WInt (denote ins n n)
+          ∗ (i, r) ↦ᵣ WInt n
+          ∗ (i, dst) ↦ᵣ WInt (denote ins n n)
       }}}.
   Proof.
     iIntros (Hdecode Hinstr Hpc_a Hvpc ϕ) "(HPC & Hpc_a & Hr & Hdst) Hφ".
     iDestruct (map_of_regs_3 with "HPC Hr Hdst") as "[Hmap (%&%&%)]".
-    iApply (wp_AddSubLt with "[$Hmap Hpc_a]"); eauto; simplify_map_eq; eauto.
-    by erewrite regs_of_is_AddSubLt; eauto; rewrite !dom_insert; set_solver+.
+    iApply (wp_AddSubLt with "[$Hmap Hpc_a]"); eauto; simplify_map_eq by simplify_pair_eq; eauto.
+    by erewrite regs_of_core_is_AddSubLt; eauto; rewrite !dom_insert; set_solver+.
     iNext. iIntros (regs' retv) "(#Hspec & Hpc_a & Hmap)". iDestruct "Hspec" as %Hspec.
 
     destruct Hspec as [| * Hfail].
     { (* Success *)
-      iApply "Hφ". iFrame. incrementPC_inv; simplify_map_eq.
-      rewrite (insert_commute _ PC dst) // insert_insert (insert_commute _ r dst) //
-              (insert_commute _ PC dst) // insert_insert.
+      iApply "Hφ". iFrame. incrementPC_inv; simplify_map_eq by simplify_pair_eq.
+      rewrite (insert_commute _ (i, PC) (i, dst)) ; simplify_pair_eq.
+      rewrite insert_insert.
+      rewrite (insert_commute _ (i, r) (i, dst)) ; simplify_pair_eq.
+      rewrite (insert_commute _ (i, PC) (i, dst)) ; simplify_pair_eq.
+      rewrite insert_insert.
       iDestruct (regs_of_map_3 with "Hmap") as "(?&?&?)"; eauto; iFrame. }
     { (* Failure (contradiction) *)
-      destruct Hfail; try incrementPC_inv; simplify_map_eq; eauto. congruence. }
+      destruct Hfail; try incrementPC_inv; simplify_map_eq by simplify_pair_eq; eauto. congruence. }
   Qed.
 
-  Lemma wp_add_sub_lt_success_dst_z E dst pc_p pc_b pc_e pc_a w ins n1 n2 pc_a' :
+  Lemma wp_add_sub_lt_success_dst_z E i dst pc_p pc_b pc_e pc_a w ins n1 n2 pc_a' :
     decodeInstrW w = ins →
     is_AddSubLt ins dst (inr dst) (inl n2) →
     (pc_a + 1)%a = Some pc_a' →
     isCorrectPC (WCap pc_p pc_b pc_e pc_a) ->
 
-    {{{ PC ↦ᵣ WCap pc_p pc_b pc_e pc_a
+    {{{ (i, PC) ↦ᵣ WCap pc_p pc_b pc_e pc_a
         ∗ pc_a ↦ₐ w
-        ∗ dst ↦ᵣ WInt n1
+        ∗ (i, dst) ↦ᵣ WInt n1
     }}}
-      Instr Executable @ E
-      {{{ RET NextIV;
-          PC ↦ᵣ WCap pc_p pc_b pc_e pc_a'
+      (i, Instr Executable) @ E
+      {{{ RET (i, NextIV);
+          (i, PC) ↦ᵣ WCap pc_p pc_b pc_e pc_a'
           ∗ pc_a ↦ₐ w
-          ∗ dst ↦ᵣ WInt (denote ins n1 n2)
+          ∗ (i, dst) ↦ᵣ WInt (denote ins n1 n2)
       }}}.
   Proof.
     iIntros (Hdecode Hinstr Hpc_a Hvpc ϕ) "(HPC & Hpc_a & Hdst) Hφ".
     iDestruct (map_of_regs_2 with "HPC Hdst") as "[Hmap %]".
-    iApply (wp_AddSubLt with "[$Hmap Hpc_a]"); eauto; simplify_map_eq; eauto.
-    by erewrite regs_of_is_AddSubLt; eauto; rewrite !dom_insert; set_solver+.
+    iApply (wp_AddSubLt with "[$Hmap Hpc_a]"); eauto; simplify_map_eq by simplify_pair_eq; eauto.
+    by erewrite regs_of_core_is_AddSubLt; eauto; rewrite !dom_insert; set_solver+.
     iNext. iIntros (regs' retv) "(#Hspec & Hpc_a & Hmap)". iDestruct "Hspec" as %Hspec.
 
     destruct Hspec as [| * Hfail].
     { (* Success *)
-      iApply "Hφ". iFrame. incrementPC_inv; simplify_map_eq.
-      rewrite (insert_commute _ PC dst) // insert_insert insert_commute // insert_insert.
+      iApply "Hφ". iFrame. incrementPC_inv; simplify_map_eq by simplify_pair_eq.
+      rewrite (insert_commute _ (i, PC) (i, dst)) ; simplify_pair_eq.
+      rewrite insert_insert.
+      rewrite insert_commute ; simplify_pair_eq.
+      rewrite insert_insert.
       iDestruct (regs_of_map_2 with "Hmap") as "(?&?)"; eauto; iFrame. }
     { (* Failure (contradiction) *)
-      destruct Hfail; try incrementPC_inv; simplify_map_eq; eauto. congruence. }
+      destruct Hfail; try incrementPC_inv; simplify_map_eq by simplify_pair_eq; eauto. congruence. }
   Qed.
 
-  Lemma wp_add_sub_lt_success_z_dst E dst pc_p pc_b pc_e pc_a w ins n1 n2 pc_a' :
+  Lemma wp_add_sub_lt_success_z_dst E i dst pc_p pc_b pc_e pc_a w ins n1 n2 pc_a' :
     decodeInstrW w = ins →
     is_AddSubLt ins dst (inl n1) (inr dst) →
     (pc_a + 1)%a = Some pc_a' →
     isCorrectPC (WCap pc_p pc_b pc_e pc_a) ->
 
-    {{{ PC ↦ᵣ WCap pc_p pc_b pc_e pc_a
+    {{{ (i, PC) ↦ᵣ WCap pc_p pc_b pc_e pc_a
         ∗ pc_a ↦ₐ w
-        ∗ dst ↦ᵣ WInt n2
+        ∗ (i, dst) ↦ᵣ WInt n2
     }}}
-      Instr Executable @ E
-      {{{ RET NextIV;
-          PC ↦ᵣ WCap pc_p pc_b pc_e pc_a'
+      (i, Instr Executable) @ E
+      {{{ RET (i, NextIV);
+          (i, PC) ↦ᵣ WCap pc_p pc_b pc_e pc_a'
           ∗ pc_a ↦ₐ w
-          ∗ dst ↦ᵣ WInt (denote ins n1 n2)
+          ∗ (i, dst) ↦ᵣ WInt (denote ins n1 n2)
       }}}.
   Proof.
     iIntros (Hdecode Hinstr Hpc_a Hvpc ϕ) "(HPC & Hpc_a & Hdst) Hφ".
     iDestruct (map_of_regs_2 with "HPC Hdst") as "[Hmap %]".
-    iApply (wp_AddSubLt with "[$Hmap Hpc_a]"); eauto; simplify_map_eq; eauto.
-    by erewrite regs_of_is_AddSubLt; eauto; rewrite !dom_insert; set_solver+.
+    iApply (wp_AddSubLt with "[$Hmap Hpc_a]"); eauto; simplify_map_eq by simplify_pair_eq; eauto.
+    by erewrite regs_of_core_is_AddSubLt; eauto; rewrite !dom_insert; set_solver+.
     iNext. iIntros (regs' retv) "(#Hspec & Hpc_a & Hmap)". iDestruct "Hspec" as %Hspec.
 
     destruct Hspec as [| * Hfail].
     { (* Success *)
-      iApply "Hφ". iFrame. incrementPC_inv; simplify_map_eq.
-      rewrite (insert_commute _ PC dst) // insert_insert insert_commute // insert_insert.
+      iApply "Hφ". iFrame. incrementPC_inv; simplify_map_eq by simplify_pair_eq.
+      rewrite (insert_commute _ (i, PC) (i, dst)) ; simplify_pair_eq.
+      rewrite insert_insert.
+      rewrite insert_commute ; simplify_pair_eq.
+      rewrite insert_insert.
       iDestruct (regs_of_map_2 with "Hmap") as "(?&?)"; eauto; iFrame. }
     { (* Failure (contradiction) *)
-      destruct Hfail; try incrementPC_inv; simplify_map_eq; eauto. congruence. }
+      destruct Hfail; try incrementPC_inv; simplify_map_eq by simplify_pair_eq; eauto. congruence. }
   Qed.
 
-  Lemma wp_add_sub_lt_success_dst_r E dst pc_p pc_b pc_e pc_a w ins n1 r2 n2 pc_a' :
+  Lemma wp_add_sub_lt_success_dst_r E i dst pc_p pc_b pc_e pc_a w ins n1 r2 n2 pc_a' :
     decodeInstrW w = ins →
     is_AddSubLt ins dst (inr dst) (inr r2) →
     (pc_a + 1)%a = Some pc_a' →
     isCorrectPC (WCap pc_p pc_b pc_e pc_a) ->
 
-    {{{ PC ↦ᵣ WCap pc_p pc_b pc_e pc_a
+    {{{ (i, PC) ↦ᵣ WCap pc_p pc_b pc_e pc_a
         ∗ pc_a ↦ₐ w
-        ∗ r2 ↦ᵣ WInt n2
-        ∗ dst ↦ᵣ WInt n1
+        ∗ (i, r2) ↦ᵣ WInt n2
+        ∗ (i, dst) ↦ᵣ WInt n1
     }}}
-      Instr Executable @ E
-      {{{ RET NextIV;
-          PC ↦ᵣ WCap pc_p pc_b pc_e pc_a'
+      (i, Instr Executable) @ E
+      {{{ RET (i, NextIV);
+          (i, PC) ↦ᵣ WCap pc_p pc_b pc_e pc_a'
           ∗ pc_a ↦ₐ w
-          ∗ r2 ↦ᵣ WInt n2
-          ∗ dst ↦ᵣ WInt (denote ins n1 n2)
+          ∗ (i, r2) ↦ᵣ WInt n2
+          ∗ (i, dst) ↦ᵣ WInt (denote ins n1 n2)
       }}}.
   Proof.
     iIntros (Hdecode Hinstr Hpc_a Hvpc ϕ) "(HPC & Hpc_a & Hr2 & Hdst) Hφ".
     iDestruct (map_of_regs_3 with "HPC Hr2 Hdst") as "[Hmap (%&%&%)]".
-    iApply (wp_AddSubLt with "[$Hmap Hpc_a]"); eauto; simplify_map_eq; eauto.
-    by erewrite regs_of_is_AddSubLt; eauto; rewrite !dom_insert; set_solver+.
+    iApply (wp_AddSubLt with "[$Hmap Hpc_a]"); eauto; simplify_map_eq by simplify_pair_eq; eauto.
+    by erewrite regs_of_core_is_AddSubLt; eauto; rewrite !dom_insert; set_solver+.
     iNext. iIntros (regs' retv) "(#Hspec & Hpc_a & Hmap)". iDestruct "Hspec" as %Hspec.
 
     destruct Hspec as [| * Hfail].
     { (* Success *)
-      iApply "Hφ". iFrame. incrementPC_inv; simplify_map_eq.
-      rewrite (insert_commute _ PC dst) // insert_insert (insert_commute _ r2 dst) //
-              (insert_commute _ PC dst) // insert_insert. 
+      iApply "Hφ". iFrame. incrementPC_inv; simplify_map_eq by simplify_pair_eq.
+      rewrite (insert_commute _ (i, PC) (i, dst)) ; simplify_pair_eq.
+      rewrite insert_insert.
+      rewrite (insert_commute _ (i, r2) (i, dst)) ; simplify_pair_eq.
+      rewrite (insert_commute _ (i, PC) (i, dst)) ; simplify_pair_eq.
+      rewrite insert_insert.
       iDestruct (regs_of_map_3 with "Hmap") as "(?&?&?)"; eauto; iFrame. }
     { (* Failure (contradiction) *)
-      destruct Hfail; try incrementPC_inv; simplify_map_eq; eauto. congruence. }
+      destruct Hfail; try incrementPC_inv; simplify_map_eq by simplify_pair_eq; eauto. congruence. }
   Qed.
 
-  Lemma wp_add_sub_lt_success_r_dst E dst pc_p pc_b pc_e pc_a w ins r1 n1 n2 pc_a' :
+  Lemma wp_add_sub_lt_success_r_dst E i dst pc_p pc_b pc_e pc_a w ins r1 n1 n2 pc_a' :
     decodeInstrW w = ins →
     is_AddSubLt ins dst (inr r1) (inr dst) →
     (pc_a + 1)%a = Some pc_a' →
     isCorrectPC (WCap pc_p pc_b pc_e pc_a) ->
 
-    {{{ PC ↦ᵣ WCap pc_p pc_b pc_e pc_a
+    {{{ (i, PC) ↦ᵣ WCap pc_p pc_b pc_e pc_a
         ∗ pc_a ↦ₐ w
-        ∗ r1 ↦ᵣ WInt n1
-        ∗ dst ↦ᵣ WInt n2
+        ∗ (i, r1) ↦ᵣ WInt n1
+        ∗ (i, dst) ↦ᵣ WInt n2
     }}}
-      Instr Executable @ E
-      {{{ RET NextIV;
-          PC ↦ᵣ WCap pc_p pc_b pc_e pc_a'
+      (i, Instr Executable) @ E
+      {{{ RET (i, NextIV);
+          (i, PC) ↦ᵣ WCap pc_p pc_b pc_e pc_a'
           ∗ pc_a ↦ₐ w
-          ∗ r1 ↦ᵣ WInt n1
-          ∗ dst ↦ᵣ WInt (denote ins n1 n2)
+          ∗ (i, r1) ↦ᵣ WInt n1
+          ∗ (i, dst) ↦ᵣ WInt (denote ins n1 n2)
       }}}.
   Proof.
     iIntros (Hdecode Hinstr Hpc_a Hvpc ϕ) "(HPC & Hpc_a & Hr2 & Hdst) Hφ".
     iDestruct (map_of_regs_3 with "HPC Hr2 Hdst") as "[Hmap (%&%&%)]".
-    iApply (wp_AddSubLt with "[$Hmap Hpc_a]"); eauto; simplify_map_eq; eauto.
-    by erewrite regs_of_is_AddSubLt; eauto; rewrite !dom_insert; set_solver+.
+    iApply (wp_AddSubLt with "[$Hmap Hpc_a]"); eauto; simplify_map_eq by simplify_pair_eq; eauto.
+    by erewrite regs_of_core_is_AddSubLt; eauto; rewrite !dom_insert; set_solver+.
     iNext. iIntros (regs' retv) "(#Hspec & Hpc_a & Hmap)". iDestruct "Hspec" as %Hspec.
 
     destruct Hspec as [| * Hfail].
     { (* Success *)
-      iApply "Hφ". iFrame. incrementPC_inv; simplify_map_eq.
-      rewrite (insert_commute _ PC dst) // insert_insert (insert_commute _ r1 dst) //
-              (insert_commute _ PC dst) // insert_insert.
+      iApply "Hφ". iFrame. incrementPC_inv; simplify_map_eq by simplify_pair_eq.
+      rewrite (insert_commute _ (i, PC) (i, dst)) ; simplify_pair_eq.
+      rewrite insert_insert.
+      rewrite (insert_commute _ (i, r1) (i, dst)) ; simplify_pair_eq.
+      rewrite (insert_commute _ (i, PC) (i, dst)) ; simplify_pair_eq.
+      rewrite insert_insert.
       iDestruct (regs_of_map_3 with "Hmap") as "(?&?&?)"; eauto; iFrame. }
     { (* Failure (contradiction) *)
-      destruct Hfail; try incrementPC_inv; simplify_map_eq; eauto. congruence. }
+      destruct Hfail; try incrementPC_inv; simplify_map_eq by simplify_pair_eq; eauto. congruence. }
   Qed.
 
-  Lemma wp_add_sub_lt_success_dst_dst E dst pc_p pc_b pc_e pc_a w ins n pc_a' :
+  Lemma wp_add_sub_lt_success_dst_dst E i dst pc_p pc_b pc_e pc_a w ins n pc_a' :
     decodeInstrW w = ins →
     is_AddSubLt ins dst (inr dst) (inr dst) →
     (pc_a + 1)%a = Some pc_a' →
     isCorrectPC (WCap pc_p pc_b pc_e pc_a) ->
 
-    {{{ PC ↦ᵣ WCap pc_p pc_b pc_e pc_a
+    {{{ (i, PC) ↦ᵣ WCap pc_p pc_b pc_e pc_a
         ∗ pc_a ↦ₐ w
-        ∗ dst ↦ᵣ WInt n
+        ∗ (i, dst) ↦ᵣ WInt n
     }}}
-      Instr Executable @ E
-      {{{ RET NextIV;
-          PC ↦ᵣ WCap pc_p pc_b pc_e pc_a'
+      (i, Instr Executable) @ E
+      {{{ RET (i, NextIV);
+          (i, PC) ↦ᵣ WCap pc_p pc_b pc_e pc_a'
           ∗ pc_a ↦ₐ w
-          ∗ dst ↦ᵣ WInt (denote ins n n)
+          ∗ (i, dst) ↦ᵣ WInt (denote ins n n)
       }}}.
   Proof.
     iIntros (Hdecode Hinstr Hpc_a Hvpc ϕ) "(HPC & Hpc_a & Hdst) Hφ".
     iDestruct (map_of_regs_2 with "HPC Hdst") as "[Hmap %]".
-    iApply (wp_AddSubLt with "[$Hmap Hpc_a]"); eauto; simplify_map_eq; eauto.
-    by erewrite regs_of_is_AddSubLt; eauto; rewrite !dom_insert; set_solver+.
+    iApply (wp_AddSubLt with "[$Hmap Hpc_a]"); eauto; simplify_map_eq by simplify_pair_eq; eauto.
+    by erewrite regs_of_core_is_AddSubLt; eauto; rewrite !dom_insert; set_solver+.
     iNext. iIntros (regs' retv) "(#Hspec & Hpc_a & Hmap)". iDestruct "Hspec" as %Hspec.
 
     destruct Hspec as [| * Hfail].
     { (* Success *)
-      iApply "Hφ". iFrame. incrementPC_inv; simplify_map_eq.
-      rewrite (insert_commute _ PC dst) // insert_insert insert_commute // insert_insert.
+      iApply "Hφ". iFrame. incrementPC_inv; simplify_map_eq by simplify_pair_eq.
+      rewrite (insert_commute _ (i, PC) (i, dst)) ; simplify_pair_eq.
+      rewrite insert_insert.
+      rewrite insert_commute; simplify_pair_eq.
+      rewrite insert_insert.
       iDestruct (regs_of_map_2 with "Hmap") as "(?&?)"; eauto; iFrame. }
     { (* Failure (contradiction) *)
-      destruct Hfail; try incrementPC_inv; simplify_map_eq; eauto. congruence. }
+      destruct Hfail; try incrementPC_inv; simplify_map_eq by simplify_pair_eq; eauto. congruence. }
   Qed.
 
-  Lemma wp_add_sub_lt_fail_z_r E ins dst n1 r2 w wdst p b e a pc_p pc_b pc_e pc_a :
+  Lemma wp_add_sub_lt_fail_z_r E i ins dst n1 r2 w wdst p b e a pc_p pc_b pc_e pc_a :
     decodeInstrW w = ins →
     is_AddSubLt ins dst (inl n1) (inr r2) →
     isCorrectPC (WCap pc_p pc_b pc_e pc_a) →
-    {{{ PC ↦ᵣ WCap pc_p pc_b pc_e pc_a ∗ pc_a ↦ₐ w ∗ dst ↦ᵣ wdst ∗ r2 ↦ᵣ WCap p b e a }}}
-      Instr Executable
-            @ E
-    {{{ RET FailedV; pc_a ↦ₐ w }}}.
+    {{{ (i, PC) ↦ᵣ WCap pc_p pc_b pc_e pc_a
+        ∗ pc_a ↦ₐ w
+        ∗ (i, dst) ↦ᵣ wdst
+        ∗ (i, r2) ↦ᵣ WCap p b e a }}}
+      (i, Instr Executable) @ E
+    {{{ RET (i, FailedV); pc_a ↦ₐ w }}}.
   Proof.
     iIntros (Hdecode Hinstr Hvpc φ) "(HPC & Hpc_a & Hdst & Hr2) Hφ".
     iDestruct (map_of_regs_3 with "HPC Hdst Hr2") as "[Hmap (%&%&%)]".
-    iApply (wp_AddSubLt with "[$Hmap Hpc_a]"); eauto; simplify_map_eq; eauto.
-      by erewrite regs_of_is_AddSubLt; eauto; rewrite !dom_insert; set_solver+.
+    iApply (wp_AddSubLt with "[$Hmap Hpc_a]"); eauto; simplify_map_eq by simplify_pair_eq; eauto.
+      by erewrite regs_of_core_is_AddSubLt; eauto; rewrite !dom_insert; set_solver+.
     iNext. iIntros (regs' retv) "(#Hspec & Hpc_a & Hmap)". iDestruct "Hspec" as %Hspec.
     destruct Hspec as [* Hsucc |].
-    { (* Success (contradiction) *) simplify_map_eq. }
+    { (* Success (contradiction) *) simplify_map_eq by simplify_pair_eq. }
     { (* Failure, done *) by iApply "Hφ". }
   Qed.
 
