theories/rules.v
@@ -3,7 +3,7 @@
 (*      rules_Lea rules_Mov rules_Restrict rules_IsPtr *)
 (*      rules_Jmp rules_Jnz rules_Subseg. *)
 From cap_machine.rules Require Export
-     rules_Get rules_Load rules_Store
+     rules_Get rules_Load rules_Store rules_AddSubLt
      rules_Lea rules_Mov
      rules_Jmp rules_Subseg.
 From iris.base_logic Require Export invariants gen_heap.
